src/Narcissus/BinLib/AlignedDomainName.v
@@ -21,6 +21,7 @@ Require Import
         Fiat.Narcissus.Formats.DomainNameOpt
         Fiat.Narcissus.BinLib.AlignedByteString
         Fiat.Narcissus.BinLib.AlignWord
+        Fiat.Narcissus.BinLib.AlignedString
         Fiat.Narcissus.BinLib.AlignedDecoders
         Fiat.Narcissus.BinLib.AlignedFix
         Fiat.Common.IterateBoundedIndex
